Owl/constants.v
@@ -1,0 +1,5 @@
+Record Lattice := {
+  labels : Set;
+}.
+
+Axiom L : Lattice. 
